Cleanup

compiler/inference/inferScript.sml
@@ -3,88 +3,95 @@ open namespacePropsTheory;
 open infer_tTheory unifyTheory;
 open stringTheory ;
 open primTypesTheory;
-open ml_monadBaseTheory ml_monadBaseLib;
+
 
 val _ = new_theory "infer";
 val _ = monadsyntax.temp_add_monadsyntax()
 val _ = patternMatchesLib.ENABLE_PMATCH_CASES();
+
+(*  The inferencer uses a state monad internally to keep track of unifications at the expressions level *)
+
+(* 'a is the type of the state, 'b is the type of successful computations, and
+ * 'c is the type of exceptions *)
+
+val _ = Datatype `
+  exc = Success 'a | Failure 'b`;
+
+val _ = type_abbrev("M", ``:'a -> ('b, 'c) exc # 'a``);
+
+val st_ex_bind_def = Define `
+(st_ex_bind : (α, β, γ) M -> (β -> (α, δ, γ) M) -> (α, δ, γ) M) x f =
+  λs.
+    dtcase x s of
+      (Success y,s) => f y s
+    | (Failure x,s) => (Failure x,s)`;
+
+val st_ex_return_def = Define `
+(st_ex_return (*: α -> (β, α, γ) M*)) x =
+  λs. (Success x, s)`;
 
 val _ = temp_overload_on ("monad_bind", ``st_ex_bind``);
 val _ = temp_overload_on ("monad_unitbind", ``\x y. st_ex_bind x (\z. y)``);
 val _ = temp_overload_on ("monad_ignore_bind", ``\x y. st_ex_bind x (\z. y)``);
 val _ = temp_overload_on ("return", ``st_ex_return``);
 
-val _ = hide "state";
+val failwith_def = Define `
+(failwith : locs option -> α -> (β, γ, (locs option # α)) M) l msg = (\s. (Failure (l, msg), s))`;
 
-(*  The inferencer uses a state monad internally to keep track of unifications at the expressions level *)
+val guard_def = Define `
+guard P l msg = if P then return () else failwith l msg`;
 
-val _ = Hol_datatype `
-  infer_exn = Exc of locs option # mlstring`;
+val read_def = Define `
+(read : (α, α, β) M) =
+  \s. (Success s, s)`;
+
+val write_def = Define `
+(write : α -> (α, unit, β) M) v =
+  \s. (Success (), v)`;
+
+val lookup_st_ex_def = Define `
+  lookup_st_ex l id ienv st =
+    dtcase nsLookup ienv id of
+    | NONE => (Failure (l, concat [implode "Undefined variable: "; id_to_string id]), st)
+    | SOME v => (Success v, st)`;
 
 val _ = Hol_datatype `
 infer_st = <| next_uvar : num;
-              subst : (num |-> infer_t) |>`;
-
-val [(_, get_next_uvar_def, set_next_uvar_def),
-     (_, get_subst_def, set_subst_def)] = define_monad_access_funs ``:infer_st``;
-
-val [(raise_Exc_def, handle_Exc_def)]  = define_monad_exception_functions ``:infer_exn`` ``:infer_st``;
-
-val _ = temp_overload_on ("failwith", ``raise_Exc``);
-
-val guard_def = Define `
-guard P l msg = if P then return () else failwith (l, msg)`;
-
-val lookup_st_ex_def = Define `
-  lookup_st_ex (l : locs option) id ienv =
-    dtcase nsLookup ienv id of
-    | NONE => failwith (l, concat [implode "Undefined variable: "; id_to_string id])
-    | SOME v => return v`;
+              subst : 'a |>`;
 
 val fresh_uvar_def = Define `
-(fresh_uvar () : (infer_st, infer_t, infer_exn) M) =
-  do uvar <- get_next_uvar;
-     set_next_uvar (uvar + 1);
-     return (Infer_Tuvar uvar)
-  od`;
+(fresh_uvar : ('b infer_st, infer_t, α) M) =
+  \s. (Success (Infer_Tuvar s.next_uvar), s with <| next_uvar := s.next_uvar + 1 |>)`;
 
 val n_fresh_uvar_def = Define  `
 n_fresh_uvar (n:num) =
   if n = 0 then
     return []
   else
-    do v <- fresh_uvar ();
+    do v <- fresh_uvar;
        vs <- n_fresh_uvar (n - 1);
        return (v::vs)
     od`;
 
 val init_infer_state_def = Define `
-  (init_infer_state : infer_st) = <| next_uvar := 0; subst := FEMPTY |>`;
+  (init_infer_state : (num |-> infer_t) infer_st) = <| next_uvar := 0; subst := FEMPTY |>`;
 
 val init_state_def = Define `
-init_state () =
-  do
-      set_next_uvar 0;
-      set_subst FEMPTY;
-      return ()
-  od`;
+init_state =
+  \st.
+    (Success (), init_infer_state)`;
 
 val add_constraint_def = Define `
 add_constraint (l : locs option) t1 t2 =
-  do
-    subst <- get_subst;
-    dtcase t_unify subst t1 t2 of
+  \st.
+    dtcase t_unify st.subst t1 t2 of
       | NONE =>
-          failwith (l, concat [implode "Type mismatch between ";
-                               inf_type_to_string (t_walkstar subst t1);
+          (Failure (l, concat [implode "Type mismatch between ";
+                               inf_type_to_string (t_walkstar st.subst t1);
                                implode " and ";
-                               inf_type_to_string (t_walkstar subst t2)])
+                               inf_type_to_string (t_walkstar st.subst t2)]), st)
       | SOME s =>
-          do
-	      set_subst s;
-              return ()
-          od
-  od`;
+          (Success (), st with <| subst := s |>)`;
 
 val add_constraints_def = Define `
 (add_constraints l [] [] =
@@ -95,18 +102,22 @@ val add_constraints_def = Define `
      return ()
   od) ∧
 (add_constraints l _ _ =
-  failwith (l, (implode "Internal error: Bad call to add_constraints")))`;
+  failwith l (implode "Internal error: Bad call to add_constraints"))`;
+
+val get_next_uvar_def = Define `
+get_next_uvar =
+  \st. (Success st.next_uvar, st)`;
 
 val apply_subst_def = Define `
 apply_subst t =
-  do subst <- get_subst;
-     return (t_walkstar subst t)
+  do st <- read;
+     return (t_walkstar st.subst t)
   od`;
 
 val apply_subst_list_def = Define `
 apply_subst_list ts =
-  do subst <- get_subst;
-     return (MAP (t_walkstar subst) ts)
+  do st <- read;
+     return (MAP (t_walkstar st.subst) ts)
   od`;
 
 (* We use a state argument for the inferencer's typing environment. This corresponds to the type system's typing environment
@@ -180,11 +191,11 @@ val infer_deBruijn_subst_def = tDefine "infer_deBruijn_subst" `
 
 val infer_p_def = tDefine "infer_p" `
 (infer_p l ienv (Pvar n) =
-  do t <- fresh_uvar();
+  do t <- fresh_uvar;
      return (t, [(n,t)])
   od) ∧
 (infer_p l ienv Pany =
-  do t <- fresh_uvar();
+  do t <- fresh_uvar;
      return (t, [])
   od) ∧
 (infer_p l ienv (Plit (IntLit i)) =
@@ -278,7 +289,7 @@ constrain_op l op ts =
           return (Infer_Tapp [] (TC_name (Short "bool")))
        od
    | (Opapp, [t1;t2]) =>
-       do uvar <- fresh_uvar();
+       do uvar <- fresh_uvar;
           () <- add_constraint l t1 (Infer_Tapp [t2;uvar] TC_fn);
           return uvar
        od
@@ -288,7 +299,7 @@ constrain_op l op ts =
        od
    | (Opref, [t]) => return (Infer_Tapp [t] TC_ref)
    | (Opderef, [t]) =>
-       do uvar <- fresh_uvar();
+       do uvar <- fresh_uvar;
           () <- add_constraint l t (Infer_Tapp [uvar] TC_ref);
           return uvar
        od
@@ -383,18 +394,18 @@ constrain_op l op ts =
           return (Infer_Tapp [] TC_string)
         od
    | (VfromList, [t]) =>
-       do uvar <- fresh_uvar();
+       do uvar <- fresh_uvar;
           () <- add_constraint l t (Infer_Tapp [uvar] (TC_name (Short "list")));
           return (Infer_Tapp [uvar] TC_vector)
        od
    | (Vsub, [t1;t2]) =>
-       do uvar <- fresh_uvar();
+       do uvar <- fresh_uvar;
           () <- add_constraint l t1 (Infer_Tapp [uvar] TC_vector);
           () <- add_constraint l t2 (Infer_Tapp [] TC_int);
           return uvar
        od
    | (Vlength, [t]) =>
-       do uvar <- fresh_uvar();
+       do uvar <- fresh_uvar;
           () <- add_constraint l t (Infer_Tapp [uvar] TC_vector);
           return (Infer_Tapp [] TC_int)
        od
@@ -403,18 +414,18 @@ constrain_op l op ts =
           return (Infer_Tapp [t2] TC_array)
        od
    | (AallocEmpty, [t1]) =>
-       do uvar <- fresh_uvar();
+       do uvar <- fresh_uvar;
           () <- add_constraint l t1 (Infer_Tapp [] TC_tup);
           return (Infer_Tapp [uvar] TC_array)
        od
    | (Asub, [t1;t2]) =>
-       do uvar <- fresh_uvar();
+       do uvar <- fresh_uvar;
           () <- add_constraint l t1 (Infer_Tapp [uvar] TC_array);
           () <- add_constraint l t2 (Infer_Tapp [] TC_int);
           return uvar
        od
    | (Alength, [t]) =>
-       do uvar <- fresh_uvar();
+       do uvar <- fresh_uvar;
           () <- add_constraint l t (Infer_Tapp [uvar] TC_array);
           return (Infer_Tapp [] TC_int)
        od
@@ -428,7 +439,7 @@ constrain_op l op ts =
           () <- add_constraint l t2 (Infer_Tapp [] TC_word8array);          
           return (Infer_Tapp [] TC_tup)
        od
-   | _ => failwith(l, (implode "Wrong number of arguments to primitive"))`;
+   | _ => failwith l (implode "Wrong number of arguments to primitive")`;
 
 val constrain_op_def = Define constrain_op_quotation
 
@@ -444,12 +455,12 @@ val infer_e_def = tDefine "infer_e" `
 (infer_e l ienv (Raise e) =
   do t2 <- infer_e l ienv e;
      () <- add_constraint l t2 (Infer_Tapp [] TC_exn);
-     t1 <- fresh_uvar ();
+     t1 <- fresh_uvar;
      return t1
   od) ∧
 (infer_e l ienv (Handle e pes) =
   if pes = [] then
-    failwith (l, (implode "Empty pattern match"))
+    failwith l (implode "Empty pattern match")
   else
     do t1 <- infer_e l ienv e;
        () <- infer_pes l ienv pes (Infer_Tapp [] TC_exn) t1;
@@ -488,7 +499,7 @@ val infer_e_def = tDefine "infer_e" `
           return (Infer_Tapp ts' (tid_exn_to_tc tn))
        od) ∧
 (infer_e l ienv (Fun x e) =
-  do t1 <- fresh_uvar ();
+  do t1 <- fresh_uvar;
      t2 <- infer_e l (ienv with inf_v := nsBind x (0,t1) ienv.inf_v) e;
      return (Infer_Tapp [t1;t2] TC_fn)
   od) ∧
@@ -514,10 +525,10 @@ val infer_e_def = tDefine "infer_e" `
   od) ∧
 (infer_e l ienv (Mat e pes) =
   if pes = [] then
-    failwith (l, (implode "Empty pattern match"))
+    failwith l (implode "Empty pattern match")
   else
     do t1 <- infer_e l ienv e;
-       t2 <- fresh_uvar ();
+       t2 <- fresh_uvar;
        () <- infer_pes l ienv pes t1 t2;
        return t2
   od) ∧
@@ -589,7 +600,7 @@ val infer_e_def = tDefine "infer_e" `
   od) ∧
 (infer_funs l ienv [] = return []) ∧
 (infer_funs l ienv ((f, x, e)::funs) =
-  do uvar <- fresh_uvar ();
+  do uvar <- fresh_uvar;
      t <- infer_e l (ienv with inf_v := nsBind x (0,uvar) ienv.inf_v) e;
      ts <- infer_funs l ienv funs;
      return (Infer_Tapp [uvar;t] TC_fn::ts)
@@ -599,7 +610,6 @@ val infer_e_def = tDefine "infer_e" `
                                     | INR (INR (INL (_,_,pes,_,_))) => exp3_size pes
                                     | INR (INR (INR (_,_,funs))) => exp1_size funs)` >>
  rw []);
-
 
 (* The final part of the inferencer state that appears at the decls level (and
  * above) are the declared names. The only difference from the type system is
@@ -616,7 +626,7 @@ val empty_inf_decls = Define `
 
 val infer_d_def = Define `
 (infer_d mn idecls ienv (Dlet locs p e) =
-  do () <- init_state ();
+  do () <- init_state;
      n <- get_next_uvar;
      t1 <- infer_e (SOME locs) ienv e;
      (t2,env') <- infer_p (SOME locs) ienv p;
@@ -632,7 +642,7 @@ val infer_d_def = Define `
   od) ∧
 (infer_d mn idecls ienv (Dletrec locs funs) =
   do () <- guard (ALL_DISTINCT (MAP FST funs)) (SOME locs) (implode "Duplicate function name");
-     () <- init_state ();
+     () <- init_state;
      next <- get_next_uvar;
      uvars <- n_fresh_uvar (LENGTH funs);
      env' <- return (nsAppend (alist_to_ns (list$MAP2 (\(f,x,e) uvar. (f,(0,uvar))) funs uvars)) ienv.inf_v);
@@ -703,7 +713,7 @@ val t_to_freevars_def = Define `
 (t_to_freevars (Tvar tn) =
   return [tn]) ∧
 (t_to_freevars (Tvar_db _) =
-  failwith(NONE, (implode "deBruijn index in type definition"))) ∧
+  failwith NONE (implode "deBruijn index in type definition")) ∧
 (t_to_freevars (Tapp ts tc) =
   ts_to_freevars ts) ∧
 (ts_to_freevars [] = return []) ∧
@@ -762,10 +772,10 @@ check_weak_decls decls_impl decls_spec ⇔
   list_subset decls_spec.inf_defined_types decls_impl.inf_defined_types ∧
   list_subset decls_spec.inf_defined_exns decls_impl.inf_defined_exns`;
 
-(* val check_tscheme_inst_def = Define `
+val check_tscheme_inst_def = Define `
   check_tscheme_inst _ (tvs_spec, t_spec) (tvs_impl, t_impl) ⇔
     let M =
-    do () <- init_state ();
+    do () <- init_state;
        uvs <- n_fresh_uvar tvs_impl;
        t <- return (infer_deBruijn_subst uvs t_impl);
        () <- add_constraint NONE t_spec t
@@ -773,23 +783,7 @@ check_weak_decls decls_impl decls_spec ⇔
     in
     dtcase M init_infer_state of
     | (Success _, _) => T
-    | (Failure _, _) => F `; *)
-
-val check_tscheme_inst_aux_def = Define `
-  check_tscheme_inst_aux _ (tvs_spec, t_spec) (tvs_impl, t_impl) ⇔
-    do () <- init_state();
-       uvs <- n_fresh_uvar tvs_impl;
-       t <- return (infer_deBruijn_subst uvs t_impl);
-       () <- add_constraint NONE t_spec t
-    od`
-
-val run_check_tscheme_inst_aux_def = Define
-`run_check_tscheme_inst_aux x1 x2 x3 state = run (check_tscheme_inst_aux x1 x2 x3) state`;
-
-val check_tscheme_inst_def = Define `
-check_tscheme_inst x1 x2 x3 = dtcase (run_check_tscheme_inst_aux x1 x2 x3 init_infer_state) of
-| Success _ => T
-| Failure _ => F `;
+    | (Failure _, _) => F `;
 
 val check_weak_ienv_def = Define `
   check_weak_ienv ienv_impl ienv_spec ⇔
@@ -840,24 +834,13 @@ val _ = Datatype`
   <| inf_decls : inf_decls
    ; inf_env   : inf_env|>`
 
-(* val infertype_prog_def = Define`
+val infertype_prog_def = Define`
   infertype_prog c prog =
     dtcase FST (infer_prog c.inf_decls c.inf_env prog init_infer_state) of
     | Success (new_decls, new_ienv) =>
         Success ( <| inf_decls := append_decls new_decls c.inf_decls
                 ; inf_env := extend_dec_ienv new_ienv c.inf_env |>)
-    | Failure x => Failure x`; *)
-
-val infertype_prog_aux_def = Define`
-  infertype_prog_aux c prog =
-    do
-	(new_decls, new_ienv) <- infer_prog c.inf_decls c.inf_env prog;
-        return ( <| inf_decls := append_decls new_decls c.inf_decls
-                ; inf_env := extend_dec_ienv new_ienv c.inf_env |>)
-    od`;
-
-val infertype_prog_def = Define `
-infertype_prog c prog = run (infertype_prog_aux c prog) init_infer_state`;
+    | Failure x => Failure x`;
 
 val conf = ``<| inf_decls := empty_inf_decls ; inf_env := (<|inf_v := nsEmpty; inf_c := nsEmpty ; inf_t := nsEmpty |>)|>``
 
